bleh

MapSpec/Journal.i.dfy
@@ -1,18 +1,34 @@
 include "../lib/Base/KeyType.s.dfy"
 include "../lib/Base/Message.i.dfy"
+include "../lib/Base/sequences.i.dfy"
 
 module Journal {
   import opened KeyType 
   import opened ValueMessage
+  import opened Sequences
   import UI
 
-  datatype JournalEntry = JournalInsert(key: Key, msg: Message)
+  datatype JournalEntry = JournalInsert(key: Key, value: Value)
 
   function JournalEntriesForUIOp(uiop: UI.Op) : seq<JournalEntry>
   {
     if uiop.PutOp? then
-      [JournalInsert(uiop.key, Define(uiop.value))]
+      [JournalInsert(uiop.key, uiop.value)]
     else
       []
+  }
+
+  function JournalEntriesForUIOps(uiops: seq<UI.Op>) : seq<JournalEntry>
+  {
+    if uiops == [] then
+      []
+    else
+      JournalEntriesForUIOps(DropLast(uiops))
+          + JournalEntriesForUIOp(Last(uiops))
+  }
+
+  function UIOpForJournalEntry(je: JournalEntry) : UI.Op
+  {
+    UI.PutOp(je.key, je.value)
   }
 }
