MapSpec/UIStateMachine.s.dfy
@@ -4,8 +4,8 @@ abstract module UIStateMachine {
   import _UI = UI
   type UIOp = _UI.Op
 
-  type Constants
-  type Variables
+  type Constants(!new)
+  type Variables(!new)
   predicate Init(k: Constants, s: Variables)
   predicate Next(k: Constants, s: Variables, s': Variables, uiop: UIOp)
 }
